14MachineCode/MachineCode.thy
@@ -2,7 +2,7 @@ theory MachineCode
   imports Main
 begin
 
-datatype reg = R1 | R2 | R3 | R4 | R5 | R6
+datatype reg = R1 | R2 | R3 | R4 | R5
 
 datatype mach = 
   LDI reg nat (* $R := k *)
